theory/Static_Communication_Analysis_B.thy
@@ -1035,60 +1035,6 @@ lemma isnt_path_sound: "
 sorry
 
 
-lemma isnt_send_evt_sound: "
-  \<lbrakk>
-    \<rho>\<^sub>y x\<^sub>e = Some (VClosure (Send_Evt x\<^sub>s\<^sub>c x\<^sub>m) \<rho>\<^sub>e);
-    ([[] \<mapsto> \<langle>e;Map.empty;[]\<rangle>], {}) \<rightarrow>* (\<E>', H');
-    \<E>' \<pi>\<^sub>y = Some (\<langle>LET x\<^sub>y = SYNC x\<^sub>e in e\<^sub>y;\<rho>\<^sub>y;\<kappa>\<^sub>y\<rangle>);
-    (V, C) \<Turnstile>\<^sub>e e
-  \<rbrakk> \<Longrightarrow>
-  {^Send_Evt x\<^sub>s\<^sub>c x\<^sub>m} \<subseteq> V x\<^sub>e
-"
-  apply (drule values_not_bound_sound; assumption?; auto)
-done
-
-lemma isnt_send_chan_sound: "
-  \<lbrakk>
-    \<rho>\<^sub>e x\<^sub>s\<^sub>c = Some (VChan (Ch \<pi> xC));
-    \<rho>\<^sub>y x\<^sub>e = Some (VClosure (Send_Evt x\<^sub>s\<^sub>c x\<^sub>m) \<rho>\<^sub>e);
-    \<E>' \<pi>\<^sub>y = Some (\<langle>LET x\<^sub>y = SYNC x\<^sub>e in e\<^sub>y;\<rho>\<^sub>y;\<kappa>\<^sub>y\<rangle>);
-    ([[] \<mapsto> \<langle>e;Map.empty;[]\<rangle>], {}) \<rightarrow>* (\<E>', H');
-    (V, C) \<Turnstile>\<^sub>e e
-  \<rbrakk> \<Longrightarrow> 
-  ^Chan xC \<in> V x\<^sub>s\<^sub>c
-"
- apply (frule may_be_static_eval_to_pool)
- apply (drule may_be_static_eval_preserved_under_concur_step_star[of _ _ _ ]; assumption?)
- apply (erule may_be_static_eval_pool.cases; auto)
- apply (drule spec[of _ \<pi>\<^sub>y], drule spec[of _ "\<langle>LET x\<^sub>y = SYNC x\<^sub>e in e\<^sub>y;\<rho>\<^sub>y;\<kappa>\<^sub>y\<rangle>"], simp)
- apply (erule may_be_static_eval_state.cases; auto)
- apply (erule may_be_static_eval_env.cases; auto)
- apply (drule spec[of _ x\<^sub>e], drule spec[of _ "(VClosure (Send_Evt x\<^sub>s\<^sub>c x\<^sub>m) \<rho>\<^sub>e)"]; simp)
- apply (erule conjE)
- apply (erule may_be_static_eval_value.cases; auto)
- apply (erule may_be_static_eval_env.cases; auto)
- apply (drule spec[of _ x\<^sub>s\<^sub>c], drule spec[of _ "(VChan (Ch \<pi> xC))"]; simp)
-done
-
-lemma isnt_send_site_sound: "
-  \<E>' \<pi>Sync = Some (\<langle>LET x\<^sub>y = SYNC x\<^sub>e in e\<^sub>n;\<rho>;\<kappa>\<rangle>) \<Longrightarrow>
-  \<rho> x\<^sub>e = Some (VClosure (Send_Evt x\<^sub>s\<^sub>c x\<^sub>m) \<rho>\<^sub>e) \<Longrightarrow>
-  \<rho>\<^sub>e x\<^sub>s\<^sub>c = Some (VChan (Ch \<pi>C xC)) \<Longrightarrow>
-  ([[] \<mapsto> \<langle>e;Map.empty;[]\<rangle>], {}) \<rightarrow>* (\<E>', H') \<Longrightarrow> 
-  (V, C) \<Turnstile>\<^sub>e e \<Longrightarrow>
-  may_be_static_send_node_label V e xC (NLet x\<^sub>y)
-"
- apply (unfold may_be_static_send_node_label.simps; auto)
- apply (rule exI[of _ x\<^sub>s\<^sub>c]; auto)
- apply (auto simp: isnt_send_chan_sound)
- apply (rule exI[of _ x\<^sub>m]; auto?)
- apply (rule exI[of _ x\<^sub>e]; auto?)
- apply (blast dest: isnt_send_evt_sound)
- apply (rule exI; auto?)
- apply (erule isnt_exp_sound; auto)
-done
-
-
 lemma isnt_send_path_sound: "
   is_send_path \<E>' (Ch \<pi>C xC) \<pi>Sync \<Longrightarrow>
   ([[] \<mapsto> \<langle>e;Map.empty;[]\<rangle>], {}) \<rightarrow>* (\<E>', H') \<Longrightarrow> 
